src/Iris/Instances/Lib/FUpd.lean
@@ -12,6 +12,7 @@ public import Iris.BI.Algebra
 public import Iris.Instances.IProp
 public import Iris.Instances.Lib.WSat
 public import Iris.Instances.Lib.LaterCredits
+public import Iris.BI.Plainly
 
 @[expose] public section
 
@@ -19,50 +20,179 @@ namespace Iris.FUpd
 
 open Iris OFE COFE BI Auth Lc
 
-section HasLC
-
-inductive HasLc where
-  | HasLc : HasLc
-  | HasNoLc : HasLc
-
-end HasLC
-
 section InvG
 
 class InvGpreS (GF : BundledGFunctors) where
   toWsatGpreS : WsatGpreS GF
   toLcGpreS : LcGpreS GF
 
-class InvGS_gen (hlc : HasLc) (GF : BundledGFunctors) extends InvGpreS GF where
+attribute [reducible, instance] InvGpreS.toWsatGpreS
+attribute [reducible, instance] InvGpreS.toLcGpreS
+
+class InvGS_gen (hlc : outParam Bool) (GF : BundledGFunctors)
+  extends InvGpreS GF where
   toWsatGS : WsatGS GF
   toLcGS : LcGS GF
 
 attribute [reducible, instance] InvGS_gen.toWsatGS
 attribute [reducible, instance] InvGS_gen.toLcGS
 
-abbrev InvGS := InvGS_gen HasLc.HasLc
+abbrev InvGS := InvGS_gen true
 
 end InvG
 
 section FUpd
 
-variable {GF : BundledGFunctors} [InvGS_gen hlc GF]
+variable {GF : BundledGFunctors} {hlc : Bool} [InvGS_gen hlc GF]
 
 def uPred_fupd (E1 E2 : CoPset) (P : IProp GF) : IProp GF :=
-  iprop(wsat ∗ ownE E1 -∗ le_upd_if (match hlc with | HasLc.HasLc => true | _ => false) iprop(◇ (wsat ∗ ownE E2 ∗ P)))
+  iprop(wsat ∗ ownE E1 -∗ le_upd_if hlc iprop(◇ (wsat ∗ ownE E2 ∗ P)))
 
-instance uPred_fupd_instance [InvGS GF] : FUpd (IProp GF) where
-  fupd := uPred_fupd (hlc := HasLc.HasLc)
+instance {E1 E2 : CoPset}
+  : NonExpansive (uPred_fupd (GF := GF) (hlc := hlc) E1 E2) where
+  ne {_ _ _} h := by
+    simp only [uPred_fupd]
+    refine wand_ne.ne .rfl ?_
+    refine le_upd_if_ne.ne ?_
+    refine except0_ne.ne ?_
+    refine sep_ne.ne .rfl ?_
+    refine sep_ne.ne .rfl h
+
+instance uPred_fupd_instance : FUpd (IProp GF) where
+  fupd := uPred_fupd
 
 end FUpd
 
 section Instances
 
-variable {GF : BundledGFunctors} [InvGS_gen hlc GF]
+open Std.LawfulSet
 
-instance uPred_bi_fupd : BIFUpdate (IProp GF) := sorry
+instance uPred_bi_fupd {GF : BundledGFunctors} [InvGS_gen hlc GF]
+  : BIFUpdate (IProp GF) where
+  fupd := uPred_fupd
+  subset Hsub := by
+    simp only [uPred_fupd]
+    iintro ⟨Hwsat, HE⟩
+    rw [diff_subset_decomp Hsub]
+    ihave ⟨HE1, HE2⟩ := (ownE_op (GF := GF) (disjoint_symm disjoint_diff_right)).mp $$ HE
+    imodintro; imodintro
+    isplitl [Hwsat]; iassumption
+    isplitl [HE2]; iassumption
+    iintro ⟨Hwsat, HE⟩
+    imodintro; imodintro
+    isplitl [Hwsat]; iassumption
+    ihave HE := (ownE_op (GF := GF) (disjoint_symm disjoint_diff_right)).mpr $$ [HE1 HE]
+    · isplitl [HE1] <;> iassumption
+    isplitl [HE]; iassumption
+    simp
+  except0 {E1 E2 P} := by
+    simp only [uPred_fupd]
+    iintro >H; iexact H
+  mono H := by
+    simp only [uPred_fupd]
+    iintro H ⟨Hwsat, HE⟩
+    ihave H := H $$ [Hwsat HE]; isplitl [Hwsat] <;> iassumption
+    iapply le_upd_if_mono $$ H
+    iintro >⟨H1, H2, H3⟩; imodintro
+    isplitl [H1]; iassumption
+    isplitl [H2]; iassumption
+    iapply H $$ H3
+  trans {_ _ _ _} := by
+    simp only [uPred_fupd]
+    iintro H ⟨Hwsat, HE⟩
+    iapply le_upd_if_trans
+    ihave H := H $$ [Hwsat HE]; isplitl [Hwsat] <;> iassumption
+    iapply le_upd_if_mono $$ H
+    iintro >⟨H1, H2, H3⟩
+    iapply H3 $$ [H1 H2]; isplitl [H1] <;> iassumption
+  mask_frame_r' {_ _ _ _} Hdisj := by
+    simp only [uPred_fupd]
+    iintro H ⟨Hwsat, HE⟩
+    ihave ⟨HE1, HE2⟩ := ownE_op (GF := GF) Hdisj $$ HE
+    ihave >H := H $$ [Hwsat HE1]; isplitl [Hwsat] <;> iassumption
+    imodintro
+    imod H with ⟨H1, H2, H3⟩; imodintro
+    ihave ⟨%Hdisj, HE⟩ := (ownE_op_iff (GF := GF)).mpr $$ [H2 HE2]
+    · isplitl [H2] <;> iassumption
+    isplitl [H1]; iassumption
+    isplitl [HE]; iassumption
+    iapply H3
+    ipure_intro; assumption
+  frame_r {_ _ _ _} := by
+    simp only [uPred_fupd]
+    iintro ⟨H, Hx⟩ ⟨Hwsat, HE⟩
+    ispecialize H $$ [Hwsat HE]; isplitl [Hwsat] <;> iassumption
+    ihave H := le_upd_if_frame_r (b := hlc) (GF := GF) $$ [H Hx]
+    · isplitl [H]
+      · iexact H
+      · iexact Hx
+    imod H with ⟨>⟨H1, H2, H3⟩, H4⟩; imodintro
+    imodintro
+    isplitl [H1]; iassumption
+    isplitl [H2]; iassumption
+    isplitl [H3]; iassumption
+    iassumption
 
-instance uPred_bi_fupd_sbi_no_lc : BIFUpdatePlainly (IProp GF) := sorry
+instance {GF : BundledGFunctors} [InvGS_gen hlc GF]
+  : BIUpdateFUpdate (IProp GF) where
+  fupd_of_bupd {_ _} := by
+    iintro H
+    simp only [fupd, uPred_fupd]
+    iintro ⟨Hwsat, HE⟩
+    imod H; imodintro; imodintro
+    isplitl [Hwsat]; iassumption
+    isplitl [HE]; iassumption
+    iassumption
+
+instance uPred_bi_fupd_plainly_no_lc {GF : BundledGFunctors} [INV : InvGS_gen false GF]
+  : BIFUpdatePlainly (IProp GF) where
+  fupd_plainly_mask_empty E P := by
+    simp only [fupd, uPred_fupd, le_upd_if, Bool.false_eq_true, ↓reduceIte]
+    iintro H G
+    ihave #>HP : ◇ ■ P $$ [H G]
+    · imod H $$ G with ⟨_, _, H⟩
+      iassumption
+    imodintro; imodintro
+    icases G with ⟨G1, G2⟩
+    isplitl [G1]; iassumption
+    isplitl [G2] <;> iassumption
+  fupd_plainly_keep_l E E' P Q := by
+    simp only [fupd, uPred_fupd, le_upd_if, Bool.false_eq_true, ↓reduceIte]
+    iintro ⟨H, Hx⟩ ⟨Hwsat, HE⟩
+    ihave #>HP : ◇ ■ P $$ [H Hx Hwsat HE]
+    · imod H $$ Hx [Hwsat HE] with ⟨_, _, H⟩
+      · isplitl [Hwsat] <;> iassumption
+      iexact H
+    imodintro
+    isplitl [Hwsat]; iassumption
+    isplitl [HE]; iassumption
+    isplitl [HP] <;> iassumption
+  fupd_plainly_later _ P := by
+    simp only [fupd, uPred_fupd, le_upd_if, Bool.false_eq_true, ↓reduceIte]
+    iintro H ⟨Hwsat, HE⟩
+    ihave #HP : ▷ ◇ ■ P $$ [H Hwsat HE]
+    · inext
+      imod H $$ [Hwsat HE] with ⟨_, _, H⟩
+      · isplitl [Hwsat] <;> iassumption
+      iexact H
+    imodintro
+    isplitl [Hwsat]; iassumption
+    isplitl [HE]; iassumption
+    imodintro
+    inext; imod HP; imodintro; iassumption
+  fupd_plainly_sForall_2 E P := by
+    simp only [fupd, uPred_fupd, le_upd_if, Bool.false_eq_true, ↓reduceIte]
+    iintro H ⟨Hwsat, HE⟩
+    ihave #HP : ◇ ■ sForall P $$ [H Hwsat HE]
+    · imod H $$ [Hwsat HE] with ⟨_, _, H⟩
+      · isplitl [Hwsat] <;> iassumption
+      iexact H
+    imodintro
+    imod HP; imodintro
+    isplitl [Hwsat]; iassumption
+    isplitl [HE]; iassumption
+    iclear H
+    iexact HP
 
 end Instances
 
@@ -72,40 +202,106 @@ variable {GF : BundledGFunctors} [InvGS GF]
 
 theorem lc_fupd_elim_later {E : CoPset} {P : IProp GF} :
   ⊢ £ 1 -∗ (▷ P) -∗ |={E}=> P := by
-  sorry
+  iintro Hcr HP
+  simp only [fupd, uPred_fupd]
+  iintro ⟨Hwsat, HE⟩
+  simp only [le_upd_if, ↓reduceIte]
+  iapply le_upd_later $$ Hcr
+  inext; imodintro
+  isplitl [Hwsat]; iassumption
+  isplitl [HE]; iassumption
+  iassumption
 
 theorem lc_fupd_add_later {E : CoPset} {P : IProp GF} :
   ⊢ £ 1 -∗ (|={E}=> ▷ P) -∗ |={E}=> P := by
-  sorry
+  iintro Hcr HP
+  simp only [fupd, uPred_fupd]
+  iintro ⟨Hwsat, HE⟩
+  simp only [le_upd_if, ↓reduceIte]
+  ihave >H := HP $$ [Hwsat HE]; isplitl [Hwsat] <;> iassumption
+  imod H with ⟨H1, H2, H3⟩
+  imod le_upd_later (GF := GF) $$ Hcr H3 with H3
+  imodintro; imodintro
+  isplitl [H1]; iassumption
+  isplitl [H2]; iassumption
+  iassumption
 
 theorem lc_fupd_add_laterN (n : Nat) {E : CoPset} {P : IProp GF} :
   ⊢ £ n -∗ (|={E}=> ▷^[n] P) -∗ |={E}=> P := by
-  sorry
+  induction n generalizing P with
+  | zero =>
+    iintro _ >H
+    ihave H := laterN_0.mp (PROP := IProp GF) $$ H
+    imodintro; iexact H
+  | succ n IH =>
+    iintro ⟨Hcr, Hcrs⟩ >HP
+    ihave HP := (laterN_later n (PROP := IProp GF)).mp $$ HP
+    iapply lc_fupd_add_later (GF := GF) $$ Hcr
+    ihave IH : £ n -∗ (|={E}=> ▷^[n]▷P) -∗ |={E}=> ▷P $$ []
+    · apply IH
+    iapply IH $$ Hcrs [HP]
+    imodintro; iexact HP
 
 end LaterCreditLemmas
 
 section Soundness
 
+open Std.LawfulSet
+
 variable {GF : BundledGFunctors}
 
-theorem fupd_soundness_no_lc_unfold [InvGpreS GF] {E1 E2 : CoPset} {P : IProp GF} :
-  (|={E1,E2}=> P) ⊢ |==> P := by
-  sorry
+theorem fupd_soundness_lc [InvGpreS GF] {E1 E2 : CoPset} {P : IProp GF} [Plain P] :
+ (∀ (_ : InvGS GF), ⊢ £ m -∗ |={E1,E2}=> P) → ⊢ P := by
+  intro H
+  iapply lc_soundness (GF := GF) (m := .succ m)
+  intro Hc
+  iintro ⟨Hcr, Hcrs⟩
+  simp only [fupd, uPred_fupd, le_upd_if, ↓reduceIte] at H
+  imod wsat_alloc (GF := GF) with ⟨%W, Hwsat, HE⟩
+  let LC : InvGS GF := {
+    toWsatGS := W
+    toLcGS := Hc
+  }
+  specialize H LC
+  have Hsub : E1 ⊆ ⊤ := fun _ _ => CoPset.mem_full
+  rw [diff_subset_decomp Hsub]
+  ihave ⟨HE1, HE2⟩ := (ownE_op (GF := GF) (disjoint_symm disjoint_diff_right)).mp $$ HE
+  ihave H : £ m -∗ wsat ∗ ownE E1 -∗ |==£> ◇ (wsat ∗ ownE E2 ∗ P) $$ []
+  · apply H
+  imod H $$ Hcrs [Hwsat HE2] with ⟨_, _, H⟩
+  · isplitl [Hwsat] <;> iassumption
+  iapply le_upd_later $$ Hcr [H]
+  iapply except0_into_later $$ H
 
 theorem fupd_soundness_no_lc [InvGpreS GF] {E1 E2 : CoPset} {P : IProp GF} [Plain P] :
-  (∀ (_ : InvGS_gen HasLc.HasNoLc GF), ⊢ |={E1,E2}=> P) → ⊢ P := by
-  sorry
+  (∀ (_ : InvGS_gen false GF), ⊢ £ m -∗ |={E1,E2}=> P) → ⊢ P := by
+  intro H
+  iapply lc_soundness (GF := GF) (m := .succ m)
+  intro Hc
+  iintro ⟨Hcr, Hcrs⟩
+  simp only [fupd, uPred_fupd, le_upd_if, Bool.false_eq_true, ↓reduceIte] at H
+  imod wsat_alloc (GF := GF) with ⟨%W, Hwsat, HE⟩
+  let LC : InvGS_gen false GF := {
+    toWsatGS := W
+    toLcGS := Hc
+  }
+  specialize H LC
+  have Hsub : E1 ⊆ ⊤ := fun _ _ => CoPset.mem_full
+  rw [diff_subset_decomp Hsub]
+  ihave ⟨HE1, HE2⟩ := (ownE_op (GF := GF) (disjoint_symm disjoint_diff_right)).mp $$ HE
+  ihave H : £ m -∗ wsat ∗ ownE E1 -∗ |==> ◇ (wsat ∗ ownE E2 ∗ P) $$ []
+  · apply H
+  imod H $$ Hcrs [Hwsat HE2] with ⟨_, _, H⟩
+  · isplitl [Hwsat] <;> iassumption
+  iapply le_upd_later $$ Hcr [H]
+  iapply except0_into_later $$ H
 
-theorem fupd_soundness_lc [InvGpreS GF] (m : Nat) {E1 E2 : CoPset} {P : IProp GF} [Plain P] :
-  (∀ (_ : InvGS GF), ⊢ £ m -∗ |={E1,E2}=> P) → ⊢ P := by
-  sorry
-
-theorem fupd_soundness_gen (hlc : HasLc) [InvGpreS GF]
+theorem fupd_soundness_gen (hlc : Bool) [InvGpreS GF]
   (m : Nat) {E1 E2 : CoPset} {P : IProp GF} [Plain P] :
-  (∀ (_ : InvGS_gen hlc GF), ⊢ match hlc with
-    | HasLc.HasLc => iprop(£ m -∗ |={E1,E2}=> P)
-    | HasLc.HasNoLc => iprop(|={E1,E2}=> P)) → ⊢ P := by
-  sorry
+  (∀ (_ : InvGS_gen hlc GF), ⊢ £ m -∗ |={E1,E2}=> P) → ⊢ P := by
+  cases hlc
+  · apply fupd_soundness_no_lc
+  · apply fupd_soundness_lc
 
 end Soundness
 
@@ -114,24 +310,148 @@ section StepIndexed
 variable {GF : BundledGFunctors}
 
 theorem step_fupdN_soundness_no_lc [InvGpreS GF]
-  (n : Nat) {E1 E2 : CoPset} {P : IProp GF} [Plain P] :
-  (∀ (_ : InvGS_gen HasLc.HasNoLc GF),
-    ⊢ Nat.fold n (fun _ _ Q => iprop(|={E1,E1}=> ▷ Q)) (iprop(|={E1,E2}=> P))) → ⊢ P := by
-  sorry
+  (n m : Nat) {P : IProp GF} [Plain P] :
+  (∀ (_ : InvGS_gen false GF),
+    ⊢ £ m -∗ |={⊤,∅}=> |={∅}▷=>^[n] P) → ⊢ P := by
+  intro H
+  apply (laterN_soundness (n := .succ n))
+  have : Persistent iprop(P) := plain_persistent
+  apply fupd_soundness_no_lc (E1 := ⊤) (E2 := ⊤) (m := m)
+  intro LC
+  specialize H LC
+  iintro Hcrds
+  iapply BIFUpdatePlainly.fupd_plainly_mask_empty
+  ihave H : £ m -∗ |={⊤,∅}=> n.iter (fun Q => iprop(|={∅}=> ▷ |={∅}=> Q)) P $$ []
+  · iapply H
+  clear H
+  imod H $$ Hcrds with H
+  imod step_fupdN_plain (P := P) $$ H with H
+  imodintro
+  iapply plainly_mono (laterN_later _).mpr
+  iapply laterN_plainly
+  inext
+  iapply later_plainly.mp
+  imod H with #H
+  inext
+  imodintro; iassumption
 
 theorem step_fupdN_soundness_lc [InvGpreS GF]
-  (n : Nat) {E1 E2 : CoPset} {P : IProp GF} [Plain P] :
+  (n m : Nat) {P : IProp GF} [Plain P] :
   (∀ (_ : InvGS GF),
-    ⊢ £ n -∗ Nat.fold n (fun _ _ Q => iprop(|={E1,E1}=> ▷ Q)) (iprop(|={E1,E2}=> P))) → ⊢ P := by
-  sorry
+    ⊢ £ m -∗ |={⊤,∅}=> |={∅}▷=>^[n] P) → ⊢ P := by
+  intro H
+  apply fupd_soundness_lc (E1 := ⊤) (E2 := ∅) (m := m + n)
+  intro LC
+  specialize H LC
+  iintro Hcrds
+  icases lc_split (GF := GF) $$ Hcrds with ⟨Hcr1, Hcr2⟩
+  ihave H : £ m -∗ |={⊤,∅}=> n.iter (fun Q => iprop(|={∅}=> ▷ |={∅}=> Q)) P $$ []
+  · iapply H
+  imod H $$ Hcr1 with H
+  clear H
+  istop
+  induction n with
+  | zero =>
+    simp only [Nat.iter_zero]
+    iintro ⟨_, HP⟩
+    imodintro
+    iassumption
+  | succ n IH =>
+    simp only [Nat.iter_succ]
+    iintro ⟨⟨Hcr, Hcrs⟩, >H⟩
+    imod lc_fupd_elim_later (GF := GF) $$ Hcr H with H
+    imod H
+    ihave IH : £ n ∗ n.iter (fun Q => iprop(|={∅}=> ▷ |={∅}=> Q)) P -∗ |={∅}=> P $$ []
+    · refine wand_intro ?_
+      refine sep_elim_r.trans ?_
+      exact IH
+    iapply IH $$ [Hcrs H]
+    isplitl [Hcrs]; iassumption
+    iassumption
 
--- theorem step_fupdN_soundness_gen (hlc : HasLc) [InvGpreS GF]
---   (n : Nat) {E1 E2 : CoPset} {P : IProp GF} [Plain P] :
---   (∀ (_ : InvGS_gen hlc GF),
---     ⊢ match hlc with
---       | HasLc.HasLc => iprop(£ n -∗ Nat.fold n (fun _ _ Q => iprop(|={E1,E1}=> ▷ Q)) iprop((|={E1,E2}=> P)))
---       | HasLc.HasNoLc => Nat.fold n (fun _ _ Q => iprop(|={E1,E1}=> ▷ Q)) iprop((|={E1,E2}=> P)) → ⊢ P) := by
---   sorry
+theorem step_fupdN_soundness_gen [InvGpreS GF]
+  (n m : Nat) {P : IProp GF} [Plain P] hlc :
+  (∀ (_ : InvGS_gen hlc GF),
+    ⊢ £ m -∗ |={⊤,∅}=> |={∅}▷=>^[n] P) → ⊢ P := by
+  cases hlc
+  · apply step_fupdN_soundness_no_lc
+  · apply step_fupdN_soundness_lc
+
+theorem step_fupdN_soundness_no_lc' [InvGpreS GF]
+  (n m : Nat) {P : IProp GF} [Plain P] :
+  (∀ (_ : InvGS_gen false GF),
+    ⊢ £ m -∗ |={⊤}[∅]▷=>^[n] P) → ⊢ P := by
+  intro H
+  apply step_fupdN_soundness_no_lc n m
+  intro LC
+  specialize H LC
+  iintro Hcr
+  cases n with
+  | zero =>
+    simp only [Nat.iter_zero] at H ⊢
+    iapply fupd_mask_intro_discard Std.LawfulSet.empty_subset
+    ihave H : £ m -∗ P $$ []
+    · apply H
+    iapply H $$ Hcr
+  | succ n =>
+    simp only [Nat.iter_succ] at H ⊢
+    ihave H : £ m -∗ |={⊤,∅}=> ▷ |={∅,⊤}=> |={⊤}[∅]▷=>^[n] P $$ []
+    · apply H
+    imod H $$ Hcr with H
+    imodintro
+    imodintro
+    inext
+    clear H
+    imod H
+    istop
+    induction n with
+    | zero =>
+      simp only [Nat.iter_zero]
+      iintro HP
+      iapply fupd_mask_intro_discard Std.LawfulSet.empty_subset
+      iassumption
+    | succ n IH =>
+      simp only [Nat.iter_succ]
+      iintro >H
+      imodintro
+      imodintro
+      inext
+      imod H
+      apply IH
+
+theorem step_fupdN_soundness_lc' [InvGpreS GF]
+  (n m : Nat) {P : IProp GF} [Plain P] :
+  (∀ (_ : InvGS GF),
+    ⊢ £ m -∗ |={⊤}[∅]▷=>^[n] P) → ⊢ P := by
+  intro H
+  apply fupd_soundness_lc (E1 := ⊤) (E2 := ⊤) (m := m + n)
+  intro LC
+  specialize H LC
+  iintro Hcrds
+  icases lc_split (GF := GF) $$ Hcrds with ⟨Hcr1, Hcr2⟩
+  ihave H : £ m -∗ |={⊤}[∅]▷=>^[n] P $$ []
+  · iapply H
+  icases H $$ Hcr1 with H
+  clear H
+  istop
+  induction n with
+  | zero =>
+    simp only [Nat.iter_zero]
+    iintro ⟨_, HP⟩
+    imodintro
+    iassumption
+  | succ n IH =>
+    simp only [Nat.iter_succ]
+    iintro ⟨⟨Hcr, Hcrs⟩, >H⟩
+    imod lc_fupd_elim_later (GF := GF) $$ Hcr H with H
+    imod H
+    ihave IH : £ n ∗ (|={⊤}[∅]▷=>^[n] P) -∗ |={⊤}=> P $$ []
+    · refine wand_intro ?_
+      refine sep_elim_r.trans ?_
+      exact IH
+    iapply IH $$ [Hcrs H]
+    isplitl [Hcrs]; iassumption
+    iassumption
 
 end StepIndexed
 
