src/Iris/Instances/Lib/Invariants.lean
@@ -10,6 +10,8 @@ public import Iris.BI.Algebra
 public import Iris.Std.Namespaces
 public import Iris.Instances.IProp
 public import Iris.Instances.Lib.FUpd
+public import Iris.Std.CoPset
+import Iris.Instances.Lib.WSat
 
 @[expose] public section
 
@@ -17,7 +19,7 @@ public import Iris.Instances.Lib.FUpd
 TODO: into_inv_inv, into_acc_inv
 -/
 
-namespace Iris.Inv
+namespace Iris
 
 open Iris OFE COFE BI FUpd
 
@@ -26,56 +28,181 @@ section InvariantDefinition
 variable {GF : BundledGFunctors} [InvGS_gen hlc GF]
 
 def inv (N : Namespace) (P : IProp GF) : IProp GF :=
-  sorry
+  iprop(□ ∀ E, ⌜↑N ⊆ E⌝ → |={E, E \ ↑N}=> ▷ P ∗ (▷ P ={E \ ↑N, E}=∗ True))
 
 def own_inv (N : Namespace) (P : IProp GF) : IProp GF :=
-  sorry
+  iprop(∃ i, ⌜i ∈ (↑N : CoPset)⌝ ∧ ownI i P)
 
 end InvariantDefinition
 
 section Instances
 
+open ProofMode
+
 variable {GF : BundledGFunctors} [InvGS_gen hlc GF]
 
-instance inv_contractive (N : Namespace) : Contractive (inv (GF := GF) N) := by
-  sorry
+instance inv_contractive (N : Namespace) : Contractive (inv (GF := GF) N) where
+  distLater_dist {n x y} H := by
+    simp only [inv]
+    refine intuitionistically_ne.ne ?_
+    refine forall_ne (fun i => ?_)
+    refine imp_ne.ne .rfl ?_
+    refine wand_ne.ne .rfl ?_
+    refine Lc.le_upd_if_ne.ne ?_
+    refine except0_ne.ne ?_
+    refine sep_ne.ne .rfl ?_
+    refine sep_ne.ne .rfl ?_
+    refine sep_ne.ne ?_ ?_
+    · exact Contractive.distLater_dist H
+    · refine wand_ne.ne ?_ .rfl
+      exact Contractive.distLater_dist H
 
-instance inv_ne (N : Namespace) : NonExpansive (inv (GF := GF) N) := by
-  sorry
+instance inv_ne (N : Namespace) : NonExpansive (inv (GF := GF) N) := ne_of_contractive _
 
 instance inv_persistent (N : Namespace) (P : IProp GF) : Persistent (inv N P) := by
-  sorry
+  simp only [inv]
+  infer_instance
 
-instance is_except_0_inv (N : Namespace) (P : IProp GF) : ProofMode.IsExcept0 (inv N P) := by
-  sorry
+instance own_inv_persistent (N : Namespace) (P : IProp GF) : Persistent (own_inv N P) := by
+  simp only [own_inv]
+  infer_instance
+
+theorem except_0_inv (N : Namespace) (P : IProp GF) :
+  ⊢ ◇ inv N P -∗ inv N P := by
+  simp only [inv]
+  iintro #H
+  imodintro
+  iintro %E %Hsub
+  imod H
+  iapply H
+  ipure_intro; assumption
+
+instance is_except_0_inv (N : Namespace) (P : IProp GF) : IsExcept0 (inv N P) where
+  is_except0 := by iintro H; iapply except_0_inv $$ H
 
 end Instances
 
 section BasicLemmas
 
+open Iris Std LawfulSet
+
 variable {GF : BundledGFunctors} [InvGS_gen hlc GF]
 
-theorem own_inv_acc (E : CoPset) (N : Namespace) (P : IProp GF) :
-  ⊢ own_inv N P -∗ |={E, E}=> ▷ P ∗ (▷ P -∗ |={E, E}=> True) := by
-  sorry
-
--- Fresh invariant name exists
--- TODO: Requires proper Namespace and Finset types
--- theorem fresh_inv_name (E : Finset Nat) (N : Namespace) :
---   ∃ i, i ∉ E ∧ i ∈ N.toSet := by
---   sorry
+theorem own_inv_acc (E : CoPset) (N : Namespace) (P : IProp GF) (Hsub : ↑N ⊆ E) :
+  ⊢ own_inv N P ={E, E \ ↑N}=∗ ▷ P ∗ (▷ P ={E \ ↑N, E}=∗ True) := by
+  simp only [own_inv, fupd, uPred_fupd]
+  iintro ⟨%i, %Hin, #Hown⟩ ⟨Hwsat, HE⟩
+  have Hsub' : ({i} : CoPset) ⊆ ↑N := by
+    intro x; simp only [mem_singleton]
+    rintro ⟨⟩
+    apply Hin
+  have HEEQ : ↑N ∪ (E \ ↑N) = E := by
+    rw [union_comm, ←diff_subset_decomp Hsub]
+  have HNEQ : {i} ∪ (nclose N \ {i}) = ↑N := by
+    rw [union_comm, ←diff_subset_decomp Hsub']
+  ihave HE : ownE (↑N ∪ (E \ ↑N)) $$ [HE]
+  · rw [HEEQ]; iexact HE
+  icases ownE_op (GF := GF) disjoint_diff_right $$ HE with ⟨HE1, HE2⟩
+  ihave HE1 : ownE ({i} ∪ (nclose N \ {i})) $$ [HE1]
+  · rw [HNEQ]; iexact HE1
+  icases ownE_op (GF := GF) disjoint_diff_right $$ HE1 with ⟨HE1, HE3⟩
+  imodintro; imodintro
+  icases ownI_open (P := P) (GF := GF) $$ [Hwsat HE1 Hown] with ⟨Hwsat, HP, HD⟩
+  · isplitl [Hwsat]; iassumption
+    isplitl [Hown]; iassumption
+    iassumption
+  isplitl [Hwsat]; iassumption
+  isplitl [HE2]; iassumption
+  isplitl [HP]; iassumption
+  iintro HP ⟨Hwsat, HE⟩
+  imodintro; imodintro
+  icases ownI_close (GF := GF) $$ [HP Hwsat HD Hown] with ⟨Hwsat, HE1⟩
+  · isplitl [Hwsat]; iassumption
+    isplitl [Hown]; iassumption
+    isplitl [HP]; iassumption
+    iassumption
+  isplitl [Hwsat]; iassumption
+  icases ownE_op (GF := GF) disjoint_diff_right $$ [HE3 HE1] with HE1
+  · isplitl [HE1]; iassumption
+    iassumption
+  rw [HNEQ]
+  icases ownE_op (GF := GF) disjoint_diff_right $$ [HE1 HE] with HE
+  · isplitl [HE1]; iassumption
+    iassumption
+  rw [HEEQ]
+  isplitl [HE]; iassumption
+  apply true_intro
 
 theorem own_inv_alloc (N : Namespace) (E : CoPset) (P : IProp GF) :
-  ⊢ ▷ P -∗ |={E}=> own_inv N P := by
-  sorry
+  ⊢ ▷ P ={E}=∗ own_inv N P := by
+  simp only [own_inv, fupd, uPred_fupd]
+  iintro HP ⟨Hw, HE⟩
+  imod ownI_alloc (.∈ (↑N : CoPset)) P $$ [HP Hw] with ⟨%i, %Hin, Hw, HI⟩
+  · intro E; apply fresh_name
+  · isplitl [Hw] <;> iassumption
+  · imodintro; imodintro
+    isplitl [Hw]; iassumption
+    isplitl [HE]; iassumption
+    iexists i
+    isplit
+    · ipure_intro; assumption
+    · iassumption
 
-theorem own_inv_alloc_open (N : Namespace) (E : CoPset) (P : IProp GF) :
-  ⊢ |={E, E}=> own_inv N P ∗ (▷ P -∗ |={E, E}=> True) := by
-  sorry
+theorem own_inv_alloc_open (N : Namespace) (E : CoPset) (P : IProp GF) (Hsub : ↑N ⊆ E) :
+  ⊢ |={E, E \ ↑N}=> own_inv N P ∗ (▷P ={E \ ↑N, E}=∗ True) := by
+  simp only [own_inv, fupd, uPred_fupd]
+  iintro ⟨Hw, HE⟩
+  imod ownI_alloc_open (φ := fun x => x ∈ (↑N : CoPset)) (P := P) (GF := GF) $$ Hw with ⟨%i, %Hin, Hcont, #HI, HD⟩
+  · intro _; apply fresh_name
+  have Hsub' : ({i} : CoPset) ⊆ ↑N := by
+    intro x; simp only [mem_singleton]
+    rintro ⟨⟩
+    apply Hin
+  have HEEQ : ↑N ∪ (E \ ↑N) = E := by
+    rw [union_comm, ←diff_subset_decomp Hsub]
+  have HNEQ : {i} ∪ (nclose N \ {i}) = ↑N := by
+    rw [union_comm, ←diff_subset_decomp Hsub']
+  ihave HE : ownE (↑N ∪ (E \ ↑N)) $$ [HE]
+  · rw [HEEQ]; iexact HE
+  icases ownE_op (GF := GF) disjoint_diff_right $$ HE with ⟨HE1, HEN⟩
+  ihave HE1 : ownE ({i} ∪ (nclose N \ {i})) $$ [HE1]
+  · rw [HNEQ]; iexact HE1
+  icases ownE_op (GF := GF) disjoint_diff_right $$ HE1 with ⟨HEi, HENi⟩
+  imodintro; imodintro
+  ispecialize Hcont $$ HEi
+  isplitl [Hcont]; iassumption
+  isplitl [HEN]; iassumption
+  isplitl [HI]
+  · iexists i; isplit
+    · ipure_intro; assumption
+    · iexact HI
+  iintro HP ⟨Hw, HE⟩
+
+  icases ownI_close (GF := GF) $$ [HP Hw HD] with ⟨Hwsat, HE1⟩
+  · isplitl [Hw]; iassumption
+    isplitl [HI]; iassumption
+    isplitl [HP]; iassumption
+    iassumption
+  imodintro; imodintro
+  isplitl [Hwsat]; iassumption
+  icases ownE_op (GF := GF) disjoint_diff_right $$ [HENi HE1] with HE1
+  · isplitl [HE1]; iassumption
+    iassumption
+  rw [HNEQ]
+  icases ownE_op (GF := GF) disjoint_diff_right $$ [HE1 HE] with HE
+  · isplitl [HE1]; iassumption
+    iassumption
+  rw [HEEQ]
+  isplitl [HE]; iassumption
+  apply true_intro
 
 theorem own_inv_to_inv (M : Namespace) (P : IProp GF) :
   ⊢ own_inv M P -∗ inv M P := by
-  sorry
+  simp only [inv]
+  iintro #I
+  imodintro
+  iintro %E %Hsub
+  iapply own_inv_acc _ _ _ Hsub (GF := GF) $$ I
 
 end BasicLemmas
 
@@ -84,31 +211,62 @@ section Allocation
 variable {GF : BundledGFunctors} [InvGS_gen hlc GF]
 
 theorem inv_alloc (N : Namespace) (E : CoPset) (P : IProp GF) :
-  ⊢ ▷ P -∗ |={E}=> inv N P := by
-  sorry
+  ⊢ ▷ P ={E}=∗ inv N P := by
+  iintro HP
+  imod own_inv_alloc N (GF := GF) $$ HP with H
+  imodintro
+  iapply own_inv_to_inv $$ H
 
-theorem inv_alloc_open (N : Namespace) (E : CoPset) (P : IProp GF) :
-  ⊢ |={E, E}=> inv N P ∗ (▷ P -∗ |={E, E}=> True) := by
-  sorry
+theorem inv_alloc_open (N : Namespace) (E : CoPset) (P : IProp GF) (Hsub : ↑N ⊆ E) :
+  ⊢ |={E, E \ ↑N}=> inv N P ∗ (▷ P ={E \ ↑N, E}=∗ True) := by
+  imod own_inv_alloc_open _ _ P Hsub (GF := GF) with ⟨Hown, Hcl⟩
+  imodintro
+  isplitr [Hcl]
+  · iapply own_inv_to_inv $$ Hown
+  · iexact Hcl
 
 end Allocation
 
 section Access
 
+open Iris Std LawfulSet
+
 variable {GF : BundledGFunctors} [InvGS_gen hlc GF]
 
-theorem inv_acc (E : CoPset) (N : Namespace) (P : IProp GF) :
-  ⊢ inv N P -∗ |={E, E}=> ▷ P ∗ (▷ P -∗ |={E, E}=> True) := by
-  sorry
+theorem inv_acc (E : CoPset) (N : Namespace) (P : IProp GF) (Hsub : ↑N ⊆ E) :
+  ⊢ inv N P ={E, E \ ↑N}=∗ ▷ P ∗ (▷ P ={E \ ↑N, E}=∗ True) := by
+  simp only [inv]
+  iintro #HI
+  iapply HI $$ %E []
+  ipure_intro; assumption
 
-theorem inv_acc_strong (E : CoPset) (N : Namespace) (P : IProp GF) :
-  ⊢ inv N P -∗ |={E, E}=>
-    ▷ P ∗ (∀ E', ▷ P -∗ |={E', E'}=> True) := by
-  sorry
+theorem inv_acc_strong (E : CoPset) (N : Namespace) (P : IProp GF) (Hsub : ↑N ⊆ E) :
+  ⊢ inv N P ={E, E \ ↑N}=∗ ▷ P ∗ ∀ E', ▷ P ={E', ↑N ∪ E'}=∗ True := by
+  iintro Hinv
+  icases inv_acc ↑N N _ subset_refl (GF := GF) $$ Hinv with H
+  rw [diff_all]
+  icases fupd_mask_frame_r disjoint_diff_right (Ef := (E \ ↑N)) (PROP := IProp GF) $$ H with H
+  rw [union_empty_left, ←union_comm (s₁ := E \ nclose N), ←diff_subset_decomp Hsub]
+  imod H with ⟨HP, H⟩
+  imodintro
+  isplitl [HP]; iassumption
+  iintro %E' HP
+  ispecialize H $$ HP
+  icases fupd_mask_frame_r disjoint_empty_left (Ef := E') (PROP := IProp GF) $$ H with H
+  rw [union_empty_left]
+  imod H
+  imodintro
+  iexact H
 
-theorem inv_acc_timeless (E : CoPset) (N : Namespace) (P : IProp GF) [Timeless P] :
-  ⊢ inv N P -∗ |={E, E}=> P ∗ (P -∗ |={E, E}=> True) := by
-  sorry
+theorem inv_acc_timeless (E : CoPset) (N : Namespace) (P : IProp GF) [Timeless P] (Hsub : ↑N ⊆ E) :
+  ⊢ inv N P ={E, E \ ↑N}=∗ P ∗ (P ={E \ ↑N, E}=∗ True) := by
+  iintro HI
+  imod inv_acc _ _ _ Hsub (GF := GF) $$ HI with ⟨>HP, H⟩
+  imodintro
+  isplitl [HP]; iassumption
+  iintro HP
+  iapply H
+  inext; iassumption
 
 end Access
 
@@ -117,26 +275,89 @@ section Modification
 variable {GF : BundledGFunctors} [InvGS_gen hlc GF]
 
 theorem inv_alter (N : Namespace) (P Q : IProp GF) :
-  ⊢ inv N P -∗ ▷ □ (P -∗ iprop(Q ∗ (Q -∗ P))) -∗ inv N Q := by
-  sorry
+  ⊢ inv N P -∗ ▷ □ (P -∗ Q ∗ (Q -∗ P)) -∗ inv N Q := by
+  simp only [inv]
+  iintro #HI #HPQ
+  imodintro
+  iintro %E Hsub
+  imod HI $$ %E Hsub with ⟨HP, H⟩
+  imodintro
+  icases HPQ $$ HP with ⟨HQ, HQP⟩
+  isplitl [HQ]
+  · iexact HQ
+  · iintro HQ
+    iapply H
+    iapply HQP $$ HQ
 
 theorem inv_iff (N : Namespace) (P Q : IProp GF) :
   ⊢ inv N P -∗ ▷ □ (P ↔ Q) -∗ inv N Q := by
-  sorry
+  iintro #HI #HPQ
+  iapply inv_alter $$ HI
+  inext; imodintro; iintro HP
+  isplitl [HP]
+  · simp only [iff]
+    ihave ⟨HPQ', _⟩ := intuitionistically_elim (PROP := IProp GF) $$ HPQ
+    iapply HPQ' $$ HP
+  · iintro HQ
+    simp only [iff]
+    ihave ⟨_, HPQ'⟩ := intuitionistically_elim (PROP := IProp GF) $$ HPQ
+    iapply HPQ' $$ HQ
 
 end Modification
 
 section Combination
 
+open Iris Std LawfulSet
+
 variable {GF : BundledGFunctors} [InvGS_gen hlc GF]
 
-theorem inv_combine (N1 N2 N : Namespace) (P Q : IProp GF) :
+theorem inv_combine (N1 N2 N : Namespace) (P Q : IProp GF) (Hdisj : N1 ## N2) (Hsub : ↑N1 ∪ ↑N2 ⊆ (↑N : CoPset)) :
   ⊢ inv N1 P -∗ inv N2 Q -∗ inv N iprop(P ∗ Q) := by
-  sorry
+  simp only [inv]
+  iintro #HI1 #HI2
+  imodintro
+  iintro %E %Hsub'
+  imod HI1 $$ %E [] with ⟨HP, H1⟩
+  · ipure_intro
+    exact subset_trans (subset_trans union_subset_left Hsub) Hsub'
+  imod HI2 $$ %(E \ ↑N1) [] with ⟨HQ, H2⟩
+  · ipure_intro
+    intro x; simp only [mem_diff]
+    specialize Hsub x; simp only [mem_union] at Hsub
+    specialize Hsub' x
+    specialize Hdisj x
+    grind
+  iapply fupd_mask_intro
+  · intro x; simp only [mem_diff, mem_diff]
+    specialize Hsub x; simp only [mem_union] at Hsub
+    specialize Hsub' x
+    specialize Hdisj x
+    grind
+  iintro Hcl
+  isplitl [HP HQ]; inext; isplitl [HP] <;> iassumption
+  iintro ⟨HP, HQ⟩
+  imod Hcl
+  imod H2 $$ HQ with _
+  imod H1 $$ HP with _
+  imodintro
+  iassumption
 
 theorem inv_combine_dup_l (N : Namespace) (P Q : IProp GF) :
-  ⊢ □ (P -∗ iprop(P ∗ P)) -∗ inv N P -∗ inv N Q -∗ inv N iprop(P ∗ Q) := by
-  sorry
+  ⊢ □ (P -∗ (P ∗ P)) -∗ inv N P -∗ inv N Q -∗ inv N iprop(P ∗ Q) := by
+  simp only [inv]
+  iintro #HPP #HI1 #HI2
+  imodintro; iintro %E #Hsub
+  imod HI1 $$ %E Hsub with ⟨HP, HI1⟩
+  ihave ⟨HP1, HP2⟩ : ▷ P ∗ ▷ P $$ [HP]
+  · iapply later_sep; inext; iapply HPP $$ HP
+  imod HI1 $$ HP2 with _
+  imod HI2 $$ %E Hsub with ⟨HQ, HI2⟩
+  imodintro
+  isplitl [HP1 HQ]
+  · inext; isplitl [HP1] <;> iassumption
+  iintro ⟨_, HQ⟩
+  imod HI2 $$ HQ with _
+  imodintro; iassumption
 
 end Combination
 
@@ -146,28 +367,33 @@ variable {GF : BundledGFunctors} [InvGS_gen hlc GF]
 
 theorem inv_split_l (N : Namespace) (P Q : IProp GF) :
   ⊢ inv N iprop(P ∗ Q) -∗ inv N P := by
-  sorry
+  iintro H
+  iapply inv_alter $$ H
+  inext; imodintro
+  iintro ⟨HP, HQ⟩
+  isplitl [HP]; iassumption
+  iintro HP
+  isplitl [HP] <;> iassumption
 
 theorem inv_split_r (N : Namespace) (P Q : IProp GF) :
   ⊢ inv N iprop(P ∗ Q) -∗ inv N Q := by
-  sorry
+  iintro H
+  iapply inv_alter $$ H
+  inext; imodintro
+  iintro ⟨HP, HQ⟩
+  isplitl [HQ]; iassumption
+  iintro HQ
+  isplitl [HP] <;> iassumption
 
 theorem inv_split (N : Namespace) (P Q : IProp GF) :
-  ⊢ inv N iprop(P ∗ Q) -∗ iprop(inv N P ∗ inv N Q) := by
-  sorry
+  ⊢ inv N iprop(P ∗ Q) -∗ inv N P ∗ inv N Q := by
+  iintro #H
+  ihave H1 := inv_split_l (GF := GF) $$ H
+  ihave H2 := inv_split_r (GF := GF) $$ H
+  isplit <;> iassumption
 
 end Splitting
 
-section Except0
-
-variable {GF : BundledGFunctors} [InvGS_gen hlc GF]
-
-theorem except_0_inv (N : Namespace) (P : IProp GF) :
-  ⊢ ◇ inv N P -∗ inv N P := by
-  sorry
-
-end Except0
-
-end Iris.Inv
+end Iris
 
 end
