src/Iris/Instances/Lib/WSat.lean
@@ -321,9 +321,9 @@ theorem ownI_alloc_open [W : WsatGS GF] (φ : Pos → Prop) (P : IProp GF)
   · unfold ownI; rw [HEQ]; isplit <;> iassumption
 
 theorem wsat_alloc [WP : WsatGpreS GF] :
-    ⊢ |==> ∃ (W : WsatGS GF), wsat (W := W) ∗ ownE CoPset.full := by
+    ⊢ |==> ∃ (W : WsatGS GF), wsat (W := W) ∗ ownE ⊤ := by
   imod (iOwn_alloc (E := WP.inv) (Auth (.own 1) empty) auth_one_valid) with ⟨%γ, H⟩
-  imod (iOwn_alloc (E := WP.enabled) (valid CoPset.full) ⟨⟩) with ⟨%γe, He⟩
+  imod (iOwn_alloc (E := WP.enabled) (valid ⊤) ⟨⟩) with ⟨%γe, He⟩
   imod (iOwn_alloc (E := WP.disabled) (valid ∅) ⟨⟩) with ⟨%γd, Hd⟩
   imodintro
   let W : WsatGS GF := {
